broken recursive traversal for gathering structures, we shouldn't go too deep

Lean/Egg/Core/Gen/StructureProjs.lean
@@ -35,3 +35,86 @@ private def buildStructureProjEqns (structName : Name) (cfg : Rewrite.Config) : 
     let rw ← Rewrite.mkDefEq lhs rhs cfg
     rws := rw :: rws
   return rws.toArray
+
+/--
+For the given rewrite (`target`), we iterate over all subterms and collect
+ `structure`s that occur in them.
+
+We use a list since we later want to `eraseDups`, but this function
+does not exist for `Array`.
+-/
+private def getStructuresInRewrite (target : Rewrite)
+   : MetaM (List Name) := do
+   for c in target.conds do
+     for ..
+  return []
+
+/--
+To generate the structure projections, we first collect all the
+structures that occur in the rewrites. For each structure, we
+generate all the projections.
+-/
+def genStructureProjections (targets : Rewrites) (norm : Config.Normalization) (cfg : Config.Erasure) :
+    MetaM Rewrites := do
+      let structures ← targets.foldlM (init := []) fun rws rw => do
+        return rws ++ (← getStructuresInRewrite rw)
+      -- deduplicate names, convert to array
+      structures.eraseDups
+       |>.foldlM  (init := #[]) fun acc struct => do
+        return acc ++ (← buildStructureProjEqns struct sorry)
+
+mutual
+/--
+We only  get the structure projcetions
+-/
+private partial def getStructuresFromConstantInfo (info : ConstantInfo) : MetaM (Array Name) :=
+  match info with
+  | .inductInfo val => do
+           match getStructureInfo? (← getEnv) val.name with
+             | none => pure #[]
+             | some structInfo => return #[structInfo.structName]
+  | .defnInfo val => getStructureNames val.value
+  | .thmInfo val => getStructureNames val.value
+  | .ctorInfo val => getStructureNames (mkConst val.name)
+  | .recInfo val => val.all.foldlM (init := #[])
+    fun structs nm => do
+      let newStructs ← getStructureNames (mkConst nm)
+      return structs ++ newStructs
+  | .quotInfo _ => pure #[]
+  | .opaqueInfo _ =>  pure #[]
+  | .axiomInfo _ => pure #[]
+
+private partial def getStructureNames (e : Expr) : MetaM (Array Name) := do
+
+  let env ← getEnv
+  let rec visit (e : Expr) (currNames : Array Name) : MetaM (Array Name) := do
+    match e with
+    | Expr.const name _ =>
+      match env.find? name with
+        | some info  => do
+          let newNames ← getStructuresFromConstantInfo info
+          return currNames ++ newNames
+        | none => pure currNames
+    | Expr.app fn arg =>
+      let fnNames ← visit fn currNames
+      let argNames ← visit arg currNames
+      return fnNames ++ argNames
+    | Expr.lam _ _ body _ =>
+      visit body currNames
+    | Expr.forallE _ _ body _ =>
+      visit body currNames
+    | Expr.mdata _ b =>
+      visit b currNames
+    | Expr.letE _ _ val body _ =>
+      let valNames ← visit val currNames
+      let bodyNames ← visit body currNames
+      return valNames ++ bodyNames
+    | _ => pure currNames
+  visit e #[]
+end  --mutual
+
+theorem foo : 1 + 1 = 2 := rfl
+
+#eval show MetaM Unit from do
+  let names ← getStructureNames (mkConst `foo)
+  trace[Meta.debug] s!"Structure names: {names}"
